
$$dZ^{\mathbb{Q}}_{u}=dZ^{\mathbb{P}}_{u}+ \frac{\mu_{u}}{\sqrt{v_{u}}}du$$

$$
\begin{align*}
S_{t}&=S_{0} \boldsymbol{\xi}\left(\int_{0}^{t}\sqrt{v_{u}} \:dZ^{\mathbb{Q}}_{u} \right) \\
& = {S_{0} \exp\left\{\int_{0}^{t}\sqrt{v_{u}} \:dZ^{\mathbb{Q}}_{u}- \frac{1}{2} \int_{0}^{t}v_{u} \:du \right\}}
\end{align*}
$$

$$
X_{0}=0
$$
$$X_{t}=\int_{0}^{t}\sqrt{v_{u}} \:dZ^{\mathbb{Q}}_{u}=\int_{0}^{t}\sqrt{v_{u}} \:(dZ^{\mathbb{P}}_{u}+\frac{\mu_{u}}{\sqrt{v_{u}}}du)=\int_{0}^{t}\mu_{u}\:du+\int_{0}^{t}\sqrt{v_{u}} \:dZ^{\mathbb{P}}_{u}$$

$$
\begin{align*}
X_{t}^{2}&=\cancelto{0}{X_{0}^{2}}+\int_{0}^{t}2X_{u} \:dX_{u}+\int_{0}^{t}v_{u} \:du \\
 & = \int_{0}^{t}2X_{u} \:(\mu_{u}du + \sqrt{v_{u}}dZ^{\mathbb{P}}_{u})+\int_{0}^{t}v_{u} \:du\\
 & = \int_{0}^{t}(2X_{u}\mu_{u}+v_{u}) \:du+\int_{0}^{t}2X_{u}\sqrt{v_{u}} \:dZ^{\mathbb{P}}_{u}
\end{align*}
$$

$$
\begin{align*}
\mathbb{E}\left[X_{t}\right] &= \cancelto{0}{\mathbb{E}\left[X_{0}\right]}+\int_{0}^{t}\mu_{u} \:du 
\end{align*}
$$

$$
\begin{align*}
\mathbb{E}\left[X_{t}^{2}\right]&=\mathbb{E}\left[\int_{0}^{t}(2X_{u}\mu_{u}+v_{u}) \:du\right]+\cancelto{0}{\mathbb{E}\left[\int_{0}^{t}2X_{u}\sqrt{v_{u}} \:dZ^{\mathbb{P}}_{u}\right]} \\
 & =\int_{0}^{t}(2\mathbb{E}\left[X_{u}\right]\mu_{u}+v_{u}) \:du\\
 & =\int_{0}^{t}\left( 2\left( \int_{0}^{u}\mu_{s} \:ds \right)\mu_{u}+v_{u} \right) \:du
\end{align*}
$$

$$
\begin{align*}
S_{t}&= S_{0} \boldsymbol{\xi}\left(\int_{0}^{t}\sqrt{v_{u}} \:dZ^{\mathbb{Q}}_{u} \right) \\
&= S_{0}\exp\left\{\int_{0}^{t}\mu_{u}\:du+\int_{0}^{t}\sqrt{v_{u}} \:dZ^{\mathbb{P}}_{u}- \frac{1}{2} \int_{0}^{t}v_{u} \:du -  \int_{0}^{t}\left( \int_{0}^{u}\mu_{s} \:ds \right)\mu_{u} \:du  \right\}\\
&= S_{0}\exp\left\{\sum I_{u}  \right\} \\
I_{u} &= \sqrt{v_{u}} \cdot dZ^{\mathbb{P}}_{u} +\left( - \frac{1}{2} v_{u} +\color{green}{\mu_{u}}+\color{orange}{\mu_{u}\left(\int_{0}^{u}\mu_{s} \:ds \right) }  \right)\cdot dt
\end{align*}
$$

$\int_{0}^{t}f(u) \:du\approx \sum f(u) \cdot du$
